zoo_parabs: Update verification.

theories/zoo_parabs/waiters.v
@@ -5,27 +5,29 @@ From zoo.language Require Import
 From zoo.diaframe Require Import
   diaframe.
 From zoo_std Require Import
-  option
-  mpsc_waiter.
+  array.
 From zoo_saturn Require Import
   mpmc_queue_1.
 From zoo_parabs Require Export
   base
   waiters__code.
+From zoo_parabs Require Import
+  waiter
+  waiters__types.
 From zoo Require Import
   options.
 
-Implicit Types b : bool.
-Implicit Types v t : val.
+Implicit Types v t waiters queue : val.
+Implicit Types 𝑤𝑎𝑖𝑡𝑒𝑟𝑠 𝑞𝑢𝑒𝑢𝑒 : list val.
 
 Class WaitersG Σ `{zoo_G : !ZooG Σ} :=
   { #[local] waiters_G_queue_G :: MpmcQueue1G Σ
-  ; #[local] waiters_G_waiter_G :: MpscWaiterG Σ
+  ; #[local] waiters_G_waiter_G :: WaiterG Σ
   }.
 
 Definition waiters_Σ := #[
   mpmc_queue_1_Σ ;
-  mpsc_waiter_Σ
+  waiter_Σ
 ].
 #[global] Instance subG_ws_hub_Σ Σ `{zoo_G : !ZooG Σ} :
   subG waiters_Σ Σ →
@@ -37,175 +39,196 @@ Qed.
 Section waiters_G.
   Context `{waiters_G : WaitersG Σ}.
 
-  #[local] Definition waiters_inv_inner t : iProp Σ :=
-    ∃ waiters,
-    mpmc_queue_1_model t waiters ∗
-    [∗ list] waiter ∈ waiters,
-      mpsc_waiter_inv waiter True.
-  Definition waiters_inv t : iProp Σ :=
-    mpmc_queue_1_inv t (nroot.@"queue") ∗
-    inv (nroot.@"inv") (waiters_inv_inner t).
+  #[local] Definition waiters_inv_inner queue : iProp Σ :=
+    ∃ 𝑞𝑢𝑒𝑢𝑒,
+    mpmc_queue_1_model queue 𝑞𝑢𝑒𝑢𝑒 ∗
+    [∗ list] 𝑤𝑎𝑖𝑡𝑒𝑟 ∈ 𝑞𝑢𝑒𝑢𝑒,
+      waiter_inv 𝑤𝑎𝑖𝑡𝑒𝑟.
+  #[local] Instance : CustomIpat "inv_inner" :=
+    " ( %𝑞𝑢𝑒𝑢𝑒
+      & >Hqueue_model
+      & H𝑞𝑢𝑒𝑢𝑒
+      )
+    ".
+  Definition waiters_inv t sz : iProp Σ :=
+    ∃ waiters 𝑤𝑎𝑖𝑡𝑒𝑟𝑠 queue,
+    ⌜t = (waiters, queue)%V⌝ ∗
+    array_model waiters Discard 𝑤𝑎𝑖𝑡𝑒𝑟𝑠 ∗
+    ⌜length 𝑤𝑎𝑖𝑡𝑒𝑟𝑠 = sz⌝ ∗
+    ([∗ list] 𝑤𝑎𝑖𝑡𝑒𝑟 ∈ 𝑤𝑎𝑖𝑡𝑒𝑟𝑠, waiter_inv 𝑤𝑎𝑖𝑡𝑒𝑟) ∗
+    mpmc_queue_1_inv queue (nroot.@"queue") ∗
+    inv (nroot.@"inv") (waiters_inv_inner queue).
+  #[local] Instance : CustomIpat "inv" :=
+    " ( %waiters
+      & %𝑤𝑎𝑖𝑡𝑒𝑟𝑠
+      & %queue
+      & ->
+      & #Hwaiters
+      & %H𝑤𝑎𝑖𝑡𝑒𝑟s
+      & #H𝑤𝑎𝑖𝑡𝑒𝑟𝑠
+      & #Hqueue_inv
+      & #Hinv
+      )
+    ".
 
-  Definition waiters_waiter t waiter : iProp Σ :=
-    mpsc_waiter_inv waiter True ∗
-    mpsc_waiter_consumer waiter.
-
-  #[global] Instance waiters_inv_persistent t :
-    Persistent (waiters_inv t).
+  #[global] Instance waiters_inv_persistent t sz :
+    Persistent (waiters_inv t sz).
   Proof.
     apply _.
   Qed.
 
-  Lemma waiters_waiter_exclusive t1 t2 waiter :
-    waiters_waiter t1 waiter -∗
-    waiters_waiter t2 waiter -∗
-    False.
-  Proof.
-    iIntros "(_ & Hwaiter_consumer1) (_ & Hwaiter_consumer2)".
-    iApply (mpsc_waiter_consumer_exclusive with "Hwaiter_consumer1 Hwaiter_consumer2").
-  Qed.
-
-  Lemma waiters_create𑁒spec :
+  Lemma waiters_create𑁒spec sz :
+    (0 ≤ sz)%Z →
     {{{
       True
     }}}
-      waiters_create ()
+      waiters_create #sz
     {{{
       t
     , RET t;
-      waiters_inv t
+      waiters_inv t ₊sz
     }}}.
   Proof.
-    iIntros "%Φ _ HΦ".
+    iIntros "%Hsz %Φ _ HΦ".
 
-    iApply wp_fupd.
+    wp_rec.
     wp_apply (mpmc_queue_1_create𑁒spec with "[//]") as (t) "(#Hqueue_inv & Hmodel)".
+
+    wp_apply (array_unsafe_init𑁒spec_disentangled (λ _ 𝑤𝑎𝑖𝑡𝑒𝑟,
+      waiter_inv 𝑤𝑎𝑖𝑡𝑒𝑟
+    )%I) as (waiters 𝑤𝑎𝑖𝑡𝑒𝑟𝑠) "(%H𝑤𝑎𝑖𝑡𝑒𝑟𝑠 & Hwaiters & H𝑤𝑎𝑖𝑡𝑒𝑟𝑠)". 1: done.
+    { iIntros "!> %i %Hi".
+      wp_apply (waiter_create𑁒spec with "[//]").
+      iSteps.
+    }
+    iMod (array_model_persist with "Hwaiters") as "#Hwaiters".
+
     iSteps.
   Qed.
 
-  #[local] Lemma waiters_notify'𑁒spec t :
+  Lemma waiters_notify_one𑁒spec t sz :
     {{{
-      waiters_inv t
+      waiters_inv t sz
     }}}
-      waiters_notify' t
+      waiters_notify_one t
     {{{
-      b
-    , RET #b;
+      RET ();
       True
     }}}.
   Proof.
-    iIntros "%Φ (#Hqueue_inv & #Hinv) HΦ".
+    iIntros "%Φ (:inv) HΦ".
 
     iLöb as "HLöb".
 
     wp_rec.
 
-    awp_apply (mpmc_queue_1_pop𑁒spec with "Hqueue_inv") without "HΦ".
-    iInv "Hinv" as "(%waiters & >Hmodel & Hwaiters)".
-    iAaccIntro with "Hmodel"; first iSteps. iIntros "Hmodel !>".
-    destruct waiters as [| waiter waiters]; first iSteps.
-    iDestruct "Hwaiters" as "(Hwaiter & Hwaiters)".
-    iSplitR "Hwaiter"; first iSteps.
+    awp_apply+ (mpmc_queue_1_pop𑁒spec with "Hqueue_inv") without "HΦ".
+    iInv "Hinv" as "(:inv_inner)".
+    iAaccIntro with "Hqueue_model". 1: iSteps. iIntros "Hqueue_model !>".
+    destruct 𝑞𝑢𝑒𝑢𝑒 as [| 𝑤𝑎𝑖𝑡𝑒𝑟 𝑞𝑢𝑒𝑢𝑒]. 1: iSteps.
+    iDestruct "H𝑞𝑢𝑒𝑢𝑒" as "(H𝑤𝑎𝑖𝑡𝑒𝑟 & H𝑞𝑢𝑒𝑢𝑒)".
+    iSplitR "H𝑤𝑎𝑖𝑡𝑒𝑟". { iFrame. }
     iIntros "_ HΦ".
 
-    wp_apply+ (mpsc_waiter_notify𑁒spec with "[$Hwaiter //]") as ([]) "_"; last iSteps.
+    wp_apply+ (waiter_notify𑁒spec with "H𝑤𝑎𝑖𝑡𝑒𝑟") as ([]) "_". 1: iSteps.
     wp_apply+ ("HLöb" with "HΦ").
   Qed.
 
-  Lemma waiters_notify𑁒spec t :
+  Lemma waiters_notify_all𑁒spec t sz :
     {{{
-      waiters_inv t
+      waiters_inv t sz
     }}}
-      waiters_notify t
+      waiters_notify_all t
     {{{
       RET ();
       True
     }}}.
   Proof.
-    iIntros "%Φ #Hinv HΦ".
+    iIntros "%Φ (:inv) HΦ".
+
+    iLöb as "HLöb".
 
     wp_rec.
-    wp_apply (waiters_notify'𑁒spec with "Hinv").
+
+    awp_apply+ (mpmc_queue_1_pop𑁒spec with "Hqueue_inv") without "HΦ".
+    iInv "Hinv" as "(:inv_inner)".
+    iAaccIntro with "Hqueue_model". 1: iSteps. iIntros "Hqueue_model !>".
+    destruct 𝑞𝑢𝑒𝑢𝑒 as [| 𝑤𝑎𝑖𝑡𝑒𝑟 𝑞𝑢𝑒𝑢𝑒]. 1: iSteps.
+    iDestruct "H𝑞𝑢𝑒𝑢𝑒" as "(H𝑤𝑎𝑖𝑡𝑒𝑟 & H𝑞𝑢𝑒𝑢𝑒)".
+    iSplitR "H𝑤𝑎𝑖𝑡𝑒𝑟". { iFrame. }
+    iIntros "_ HΦ".
+
+    wp_apply+ (waiter_notify𑁒spec with "H𝑤𝑎𝑖𝑡𝑒𝑟") as (res) "_".
+    wp_apply+ ("HLöb" with "HΦ").
+  Qed.
+
+  Lemma waiters_prepare_wait𑁒spec t (sz : nat) i :
+    (0 ≤ i < sz)%Z →
+    {{{
+      waiters_inv t sz
+    }}}
+      waiters_prepare_wait t #i
+    {{{
+      RET ();
+      True
+    }}}.
+  Proof.
+    iIntros "%Hi %Φ (:inv) HΦ".
+
+    destruct (lookup_lt_is_Some_2 𝑤𝑎𝑖𝑡𝑒𝑟𝑠 ₊i) as (𝑤𝑎𝑖𝑡𝑒𝑟 & H𝑤𝑎𝑖𝑡𝑒𝑟𝑠_lookup). 1: lia.
+    iDestruct (big_sepL_lookup with "H𝑤𝑎𝑖𝑡𝑒𝑟𝑠") as "H𝑤𝑎𝑖𝑡𝑒𝑟". 1: done.
+
+    wp_rec.
+    wp_apply+ (array_unsafe_get𑁒spec with "Hwaiters") as "_". 1-3: done || lia.
+    wp_apply+ (waiter_prepare_wait𑁒spec with "H𝑤𝑎𝑖𝑡𝑒𝑟") as "_".
+
+    awp_apply+ (mpmc_queue_1_push𑁒spec with "Hqueue_inv") without "HΦ".
+    iInv "Hinv" as "(:inv_inner)".
+    iAaccIntro with "Hqueue_model". 1: iSteps. iIntros "Hqueue_model !>".
+    iSplitL. { iFrameSteps. }
     iSteps.
   Qed.
 
-  Lemma waiters_notify_many𑁒spec t n :
-    (0 ≤ n)%Z →
+  Lemma waiters_cancel_wait𑁒spec t (sz : nat) i :
+    (0 ≤ i < sz)%Z →
     {{{
-      waiters_inv t
+      waiters_inv t sz
     }}}
-      waiters_notify_many t #n
+      waiters_cancel_wait t #i
     {{{
       RET ();
       True
     }}}.
   Proof.
-    iIntros "%Hn %Φ #Hinv HΦ".
+    iIntros "%Hi %Φ (:inv) HΦ".
 
-    iLöb as "HLöb" forall (n Hn).
-
-    wp_rec. wp_pures.
-    case_bool_decide; last iSteps.
-    wp_apply+ (waiters_notify'𑁒spec with "Hinv") as ([]) "_"; last iSteps.
-    wp_apply+ ("HLöb" with "[] HΦ"); first iSteps.
-  Qed.
-
-  Lemma waiters_prepare_wait𑁒spec t :
-    {{{
-      waiters_inv t
-    }}}
-      waiters_prepare_wait t
-    {{{
-      waiter
-    , RET waiter;
-      waiters_waiter t waiter
-    }}}.
-  Proof.
-    iIntros "%Φ (#Hqueue_inv & #Hinv) HΦ".
+    destruct (lookup_lt_is_Some_2 𝑤𝑎𝑖𝑡𝑒𝑟𝑠 ₊i) as (𝑤𝑎𝑖𝑡𝑒𝑟 & H𝑤𝑎𝑖𝑡𝑒𝑟𝑠_lookup). 1: lia.
+    iDestruct (big_sepL_lookup with "H𝑤𝑎𝑖𝑡𝑒𝑟𝑠") as "H𝑤𝑎𝑖𝑡𝑒𝑟". 1: done.
 
     wp_rec.
-    wp_apply (mpsc_waiter_create𑁒spec with "[//]") as (waiter) "(#Hwaiter_inv & Hwaiter_consumer)".
-
-    awp_apply+ (mpmc_queue_1_push𑁒spec with "Hqueue_inv") without "Hwaiter_consumer HΦ".
-    iInv "Hinv" as "(%waiters & >Hmodel & Hwaiters)".
-    iAaccIntro with "Hmodel"; first iSteps. iIntros "Hmodel !>".
-    iSplitL. { iSteps. iApply big_sepL_snoc. iSteps. }
-    iSteps.
+    wp_apply+ (array_unsafe_get𑁒spec with "Hwaiters") as "_". 1-3: done || lia.
+    wp_apply+ (waiter_cancel_wait𑁒spec with "H𝑤𝑎𝑖𝑡𝑒𝑟 HΦ").
   Qed.
 
-  Lemma waiters_cancel_wait𑁒spec t waiter :
+  Lemma waiters_commit_wait𑁒spec t (sz : nat) i :
+    (0 ≤ i < sz)%Z →
     {{{
-      waiters_inv t ∗
-      waiters_waiter t waiter
+      waiters_inv t sz
     }}}
-      waiters_cancel_wait t waiter
+      waiters_commit_wait t #i
     {{{
       RET ();
       True
     }}}.
   Proof.
-    iIntros "%Φ (#Hinv & (#Hwaiter_inv & Hwaiter_consumer)) HΦ".
+    iIntros "%Hi %Φ (:inv) HΦ".
+
+    destruct (lookup_lt_is_Some_2 𝑤𝑎𝑖𝑡𝑒𝑟𝑠 ₊i) as (𝑤𝑎𝑖𝑡𝑒𝑟 & H𝑤𝑎𝑖𝑡𝑒𝑟𝑠_lookup). 1: lia.
+    iDestruct (big_sepL_lookup with "H𝑤𝑎𝑖𝑡𝑒𝑟𝑠") as "H𝑤𝑎𝑖𝑡𝑒𝑟". 1: done.
 
     wp_rec.
-    wp_apply+ (mpsc_waiter_notify𑁒spec with "[$Hwaiter_inv //]") as ([]) "_"; last iSteps.
-    wp_apply+ (waiters_notify𑁒spec with "Hinv HΦ").
-  Qed.
-
-  Lemma waiters_commit_wait𑁒spec t waiter :
-    {{{
-      waiters_inv t ∗
-      waiters_waiter t waiter
-    }}}
-      waiters_commit_wait t waiter
-    {{{
-      RET ();
-      True
-    }}}.
-  Proof.
-    iIntros "%Φ (#Hinv & (#Hwaiter_inv & Hwaiter_consumer)) HΦ".
-
-    wp_rec.
-    wp_apply+ (mpsc_waiter_wait𑁒spec with "[$Hwaiter_inv $Hwaiter_consumer] HΦ").
+    wp_apply+ (array_unsafe_get𑁒spec with "Hwaiters") as "_". 1-3: done || lia.
+    wp_apply+ (waiter_commit_wait𑁒spec with "H𝑤𝑎𝑖𝑡𝑒𝑟 HΦ").
   Qed.
 End waiters_G.
 
@@ -213,4 +236,3 @@ From zoo_parabs Require
   waiters__opaque.
 
 #[global] Opaque waiters_inv.
-#[global] Opaque waiters_waiter.
