theories/zoo_parabs/waiters__code.v
@@ -3,54 +3,54 @@ From zoo Require Import
 From zoo.language Require Import
   typeclasses
   notations.
+From zoo_parabs Require Import
+  waiter.
 From zoo_saturn Require Import
   mpmc_queue_1.
 From zoo_std Require Import
-  mpsc_waiter.
+  array.
 From zoo_parabs Require Import
   waiters__types.
 From zoo Require Import
   options.
 
 Definition waiters_create : val :=
-  mpmc_queue_1_create.
+  fun: "sz" =>
+    (array_unsafe_init "sz" waiter_create, mpmc_queue_1_create ()).
 
-Definition waiters_notify' : val :=
-  rec: "notify'" "t" =>
-    match: mpmc_queue_1_pop "t" with
+Definition waiters_notify_one : val :=
+  rec: "notify_one" "t" =>
+    match: mpmc_queue_1_pop "t".<queue> with
     | None =>
-        false
+        ()
     | Some "waiter" =>
-        if: mpsc_waiter_notify "waiter" then (
-          "notify'" "t"
-        ) else (
-          true
+        if: ~ waiter_notify "waiter" then (
+          "notify_one" "t"
         )
     end.
 
-Definition waiters_notify : val :=
-  fun: "t" =>
-    waiters_notify' "t" ;;
-    ().
-
-Definition waiters_notify_many : val :=
-  rec: "notify_many" "t" "n" =>
-    if: 0 < "n" and waiters_notify' "t" then (
-      "notify_many" "t" ("n" - 1)
-    ).
+Definition waiters_notify_all : val :=
+  rec: "notify_all" "t" =>
+    match: mpmc_queue_1_pop "t".<queue> with
+    | None =>
+        ()
+    | Some "waiter" =>
+        waiter_notify "waiter" ;;
+        "notify_all" "t"
+    end.
 
 Definition waiters_prepare_wait : val :=
-  fun: "t" =>
-    let: "waiter" := mpsc_waiter_create () in
-    mpmc_queue_1_push "t" "waiter" ;;
-    "waiter".
+  fun: "t" "i" =>
+    let: "waiter" := array_unsafe_get "t".<waiters> "i" in
+    waiter_prepare_wait "waiter" ;;
+    mpmc_queue_1_push "t".<queue> "waiter".
 
 Definition waiters_cancel_wait : val :=
-  fun: "t" "waiter" =>
-    if: mpsc_waiter_notify "waiter" then (
-      waiters_notify "t"
-    ).
+  fun: "t" "i" =>
+    let: "waiter" := array_unsafe_get "t".<waiters> "i" in
+    waiter_cancel_wait "waiter".
 
 Definition waiters_commit_wait : val :=
-  fun: "_t" "waiter" =>
-    mpsc_waiter_wait "waiter".
+  fun: "t" "i" =>
+    let: "waiter" := array_unsafe_get "t".<waiters> "i" in
+    waiter_commit_wait "waiter".
