theories/zoo_parabs/waiters__opaque.v
@@ -2,8 +2,8 @@ From zoo_parabs Require Import
   waiters__code.
 
 #[global] Opaque waiters_create.
-#[global] Opaque waiters_notify.
-#[global] Opaque waiters_notify_many.
+#[global] Opaque waiters_notify_one.
+#[global] Opaque waiters_notify_all.
 #[global] Opaque waiters_prepare_wait.
 #[global] Opaque waiters_cancel_wait.
 #[global] Opaque waiters_commit_wait.
