theories/zoo_parabs/waiters__types.v
@@ -3,10 +3,20 @@ From zoo Require Import
 From zoo.language Require Import
   typeclasses
   notations.
+From zoo_parabs Require Import
+  waiter.
 From zoo_saturn Require Import
   mpmc_queue_1.
 From zoo_std Require Import
-  mpsc_waiter.
+  array.
 From zoo Require Import
   options.
 
+Notation "'waiters'" := (
+  in_type "zoo_parabs.waiters.t" 0
+)(in custom zoo_proj
+).
+Notation "'queue'" := (
+  in_type "zoo_parabs.waiters.t" 1
+)(in custom zoo_proj
+).
